# imports: http://www.w3.org/2004/02/skos/core

@prefix IdentifierScheme: <http://purl.bdrc.io/ontology/schemes/core/IdentifierScheme/> .
@prefix adm: <http://purl.bdrc.io/ontology/admin/> .
@prefix bda: <http://purl.bdrc.io/admindata/> .
@prefix bdo: <http://purl.bdrc.io/ontology/core/> .
@prefix bdr: <http://purl.bdrc.io/resource/> .
@prefix bf: <http://id.loc.gov/ontologies/bibframe/> .
@prefix dct: <http://purl.org/dc/terms/> .
@prefix owl: <http://www.w3.org/2002/07/owl#> .
@prefix rdf: <http://www.w3.org/1999/02/22-rdf-syntax-ns#> .
@prefix rdfs: <http://www.w3.org/2000/01/rdf-schema#> .
@prefix skos: <http://www.w3.org/2004/02/skos/core#> .
@prefix xsd: <http://www.w3.org/2001/XMLSchema#> .

<http://purl.bdrc.io/ontology/schemes/core/IdentifierScheme/>
	a owl:Ontology ;
	dct:license bda:LicenseCC0 ;
	owl:imports <http://www.w3.org/2004/02/skos/core> ;
	owl:versionInfo "Initial version"^^xsd:string ;
	.

bdo:Identifier
	a owl:Class ;
	rdfs:label "Identifier"@en ;
	skos:definition "Identifiers for Bibliographic entities, Places and other Entities"@en ;
	.

bdr:BibliographicIdentifier
	a
		bdo:Identifier ,
		skos:Concept
		;
	rdfs:subClassOf bf:Identifier ;
	rdfs:label "Bibliographic Identifer"@en ;
	skos:definition "An identifier associated with a bibliographic concept such as Work, Instance or Item"@en ;
	skos:editorialNote "extends the Bibframe 2 Identifier class"@en ;
	skos:narrower
		bdr:InstanceIdentifier ,
		bdr:ItemIdentifier ,
		bdr:WorkIdentifier
		;
	skos:topConceptOf bdr:IdentifierScheme ;
	.

bdr:CBCSiglaA
	a
		bdo:Identifier ,
		skos:Concept
		;
	rdfs:label
		"CBC Sigla A"@en ,
		"趙城金藏"@zh-hant
		;
	skos:broader bdr:CBCSiglaIdentifier ;
	skos:definition "Indicates a CBC Sigla A associated with this Instance."@en ;
	.

bdr:CBCSiglaB
	a
		bdo:Identifier ,
		skos:Concept
		;
	rdfs:label
		"CBC Sigla B"@en ,
		"大藏經補編"@zh-hant
		;
	skos:broader bdr:CBCSiglaIdentifier ;
	skos:definition "Indicates a CBC Sigla B associated with this Instance."@en ;
	.

bdr:CBCSiglaC
	a
		bdo:Identifier ,
		skos:Concept
		;
	rdfs:label
		"CBC Sigla C"@en ,
		"中華大藏經-中華書局版"@zh-hant
		;
	skos:broader bdr:CBCSiglaIdentifier ;
	skos:definition "Indicates a CBC Sigla C associated with this Instance."@en ;
	.

bdr:CBCSiglaD
	a
		bdo:Identifier ,
		skos:Concept
		;
	rdfs:label
		"CBC Sigla D"@en ,
		"國圖善本"@zh-hant
		;
	skos:broader bdr:CBCSiglaIdentifier ;
	skos:definition "Indicates a CBC Sigla D associated with this Instance."@en ;
	.

bdr:CBCSiglaF
	a
		bdo:Identifier ,
		skos:Concept
		;
	rdfs:label
		"CBC Sigla F"@en ,
		"房山石經"@zh-hant
		;
	skos:broader bdr:CBCSiglaIdentifier ;
	skos:definition "Indicates a CBC Sigla F associated with this Instance."@en ;
	.

bdr:CBCSiglaG
	a
		bdo:Identifier ,
		skos:Concept
		;
	rdfs:label
		"CBC Sigla G"@en ,
		"佛教大藏經"@zh-hant
		;
	skos:broader bdr:CBCSiglaIdentifier ;
	skos:definition "Indicates a CBC Sigla G associated with this Instance."@en ;
	.

bdr:CBCSiglaGA
	a
		bdo:Identifier ,
		skos:Concept
		;
	rdfs:label
		"CBC Sigla GA"@en ,
		"中國佛寺史志彙刊"@zh-hant
		;
	skos:broader bdr:CBCSiglaIdentifier ;
	skos:definition "Indicates a CBC Sigla GA associated with this Instance."@en ;
	.

bdr:CBCSiglaGB
	a
		bdo:Identifier ,
		skos:Concept
		;
	rdfs:label
		"CBC Sigla GB"@en ,
		"中國佛寺志叢刊"@zh-hant
		;
	skos:broader bdr:CBCSiglaIdentifier ;
	skos:definition "Indicates a CBC Sigla GB associated with this Instance."@en ;
	.

bdr:CBCSiglaI
	a
		bdo:Identifier ,
		skos:Concept
		;
	rdfs:label
		"CBC Sigla I"@en ,
		"北朝佛教石刻拓片百品"@zh-hant
		;
	skos:broader bdr:CBCSiglaIdentifier ;
	skos:definition "Indicates a CBC Sigla I associated with this Instance."@en ;
	.

bdr:CBCSiglaIdentifier
	a
		bdo:Identifier ,
		skos:Concept
		;
	rdfs:label "CBC Sigla Identifer"@en ;
	skos:broader bdr:InstanceIdentifier ;
	skos:definition "An identifier associated with a CBC Instance"@en ;
	.

bdr:CBCSiglaJ
	a
		bdo:Identifier ,
		skos:Concept
		;
	rdfs:label
		"CBC Sigla J"@en ,
		"嘉興藏"@zh-hant
		;
	skos:broader bdr:CBCSiglaIdentifier ;
	skos:definition "Indicates a CBC Sigla J associated with this Instance."@en ;
	.

bdr:CBCSiglaK
	a
		bdo:Identifier ,
		skos:Concept
		;
	rdfs:label
		"Koreana number"@en ,
		"高麗大藏經-新文豐版"@zh-hant
		;
	skos:broader bdr:CBCSiglaIdentifier ;
	skos:definition "The Koreana number, as indicated in the catalog by Lewis R. Lancaster."@en ;
	.

bdr:CBCSiglaL
	a
		bdo:Identifier ,
		skos:Concept
		;
	rdfs:label
		"CBC Sigla L"@en ,
		"乾隆大藏經-新文豐版"@zh-hant
		;
	skos:broader bdr:CBCSiglaIdentifier ;
	skos:definition "Indicates a CBC Sigla L associated with this Instance."@en ;
	.

bdr:CBCSiglaM
	a
		bdo:Identifier ,
		skos:Concept
		;
	rdfs:label
		"CBC Sigla M"@en ,
		"卍正藏經-新文豐版"@zh-hant
		;
	skos:broader bdr:CBCSiglaIdentifier ;
	skos:definition "Indicates a CBC Sigla M associated with this Instance."@en ;
	.

bdr:CBCSiglaN
	a
		bdo:Identifier ,
		skos:Concept
		;
	rdfs:label
		"CBC Sigla N"@en ,
		"南傳大藏經"@zh-hant
		;
	skos:broader bdr:CBCSiglaIdentifier ;
	skos:definition "Indicates a CBC Sigla N associated with this Instance."@en ;
	.

bdr:CBCSiglaP
	a
		bdo:Identifier ,
		skos:Concept
		;
	rdfs:label
		"CBC Sigla P"@en ,
		"永樂北藏"@zh-hant
		;
	skos:broader bdr:CBCSiglaIdentifier ;
	skos:definition "Indicates a CBC Sigla P associated with this Instance."@en ;
	.

bdr:CBCSiglaS
	a
		bdo:Identifier ,
		skos:Concept
		;
	rdfs:label
		"CBC Sigla S"@en ,
		"宋藏遺珍-新文豐版"@zh-hant
		;
	skos:broader bdr:CBCSiglaIdentifier ;
	skos:definition "Indicates a CBC Sigla S associated with this Instance."@en ;
	.

bdr:CBCSiglaT
	a
		bdo:Identifier ,
		skos:Concept
		;
	rdfs:label
		"Taisho reference number"@en ,
		"大正藏"@zh-hant
		;
	skos:broader bdr:CBCSiglaIdentifier ;
	skos:definition "Indicates the Taisho number associated with this Instance, withtout the volume number (ex: T0001, not T01n0001)."@en ;
	.

bdr:CBCSiglaU
	a
		bdo:Identifier ,
		skos:Concept
		;
	rdfs:label
		"CBC Sigla U"@en ,
		"洪武南藏"@zh-hant
		;
	skos:broader bdr:CBCSiglaIdentifier ;
	skos:definition "Indicates a CBC Sigla U associated with this Instance."@en ;
	.

bdr:CBCSiglaX
	a
		bdo:Identifier ,
		skos:Concept
		;
	rdfs:label
		"CBC Sigla X"@en ,
		"卍續藏"@zh-hant
		;
	skos:broader bdr:CBCSiglaIdentifier ;
	skos:definition "Indicates a CBC Sigla X associated with this Instance."@en ;
	.

bdr:CBCSiglaY
	a
		bdo:Identifier ,
		skos:Concept
		;
	rdfs:label
		"CBC Sigla Y"@en ,
		"印順法師佛學著作集"@zh-hant
		;
	skos:broader bdr:CBCSiglaIdentifier ;
	skos:definition "Indicates a CBC Sigla Y associated with this Instance."@en ;
	.

bdr:CBCSiglaZS
	a
		bdo:Identifier ,
		skos:Concept
		;
	rdfs:label
		"CBC Sigla ZS"@en ,
		"正史佛教資料類編"@zh-hant
		;
	skos:broader bdr:CBCSiglaIdentifier ;
	skos:definition "Indicates a CBC Sigla ZS associated with this Instance."@en ;
	.

bdr:CBCSiglaZW
	a
		bdo:Identifier ,
		skos:Concept
		;
	rdfs:label
		"CBC Sigla ZW"@en ,
		"藏外佛教文獻"@zh-hant
		;
	skos:broader bdr:CBCSiglaIdentifier ;
	skos:definition "Indicates a CBC Sigla ZW associated with this Instance."@en ;
	.

bdr:CHGISId
	a
		bdo:Identifier ,
		skos:Concept
		;
	skos:broader bdr:PlaceIdentifier ;
	skos:definition "The China Historical GIS identifier for the Place"@en ;
	skos:editorialNote 'Note that in the BDRC dataset, these are in fact invalid identifiers that conflict with other ones. The way to get the correct ID is to prefix the local name with "TBRC_", for example, "TBRC_G162".'@en ;
	skos:historyNote "Was bdo:placeChgisId."@en ;
	skos:prefLabel "chgis id"@en ;
	.

bdr:DommId
	a
		bdo:Identifier ,
		skos:Concept
		;
	skos:broader bdr:PlaceIdentifier ;
	skos:definition "The identifier used in the Documentation of Mongolian Monasteries project"@en ;
	skos:prefLabel "DOMM id"@en ;
	.

bdr:FEMCManuscriptCode
	a
		bdo:Identifier ,
		skos:Concept
		;
	skos:broader bdr:InstanceIdentifier ;
	skos:definition "Code used in the publications by the Fonds d'Édition des Manuscrits du Cambodge (FEMC), or extension of these codes by BDRC."@en ;
	skos:prefLabel "FEMC code"@en ;
	.

bdr:GB2260-2013
	a
		bdo:Identifier ,
		skos:Concept
		;
	rdfs:label "GB2260-2013"@en ;
	skos:broader bdr:PlaceIdentifier ;
	skos:definition "The 2013 Chinese GB code for the Place. Similar to U.S. Zipcode"@en ;
	skos:historyNote "Was bdo:placeGB2260-2013."@en ;
	.

bdr:HarvardShelfId
	a
		bdo:Identifier ,
		skos:Concept
		;
	skos:broader bdr:InstanceIdentifier ;
	skos:definition "Harvard Library identifier for physical items at Harvard and cataloged in BDRC"@en ;
	skos:historyNote "Was bdo:workSeeHarvard."@en ;
	skos:prefLabel "hollis shelf id"@en ;
	.

bdr:HollisId
	a
		bdo:Identifier ,
		skos:Concept
		;
	skos:broader bdr:InstanceIdentifier ;
	skos:definition "Identifier assigned by Harvard Library to BDRC digital assets on file at Harvard."@en ;
	skos:editorialNote "There may be more than one Hollis ID for a Work owing to differences in cataloguing policy between TBRC and Harvard"@en ;
	skos:historyNote "Was bdo:workHollis."@en ;
	skos:prefLabel "hollis id"@en ;
	.

bdr:IDNGMPP
	a
		bdo:Identifier ,
		skos:Concept
		;
	rdfs:label "NGMPP Reel Number"@en ;
	skos:broader bdr:InstanceIdentifier ;
	skos:definition "Indicates the NGMPP Reel Number"@en ;
	.

bdr:IdentifierScheme
	a skos:ConceptScheme ;
	skos:prefLabel "Identifier Scheme"@en ;
	.

bdr:InstanceIdentifier
	a
		bdo:Identifier ,
		skos:Concept
		;
	rdfs:label "Instance Identifer"@en ;
	skos:broader bdr:BibliographicIdentifier ;
	skos:definition "An identifier associated with an Instance"@en ;
	skos:narrower
		bdr:CBCSiglaIdentifier ,
		bdr:KaTenSiglaIdentifier
		;
	.

bdr:ItemIdentifier
	a
		bdo:Identifier ,
		skos:Concept
		;
	rdfs:label "Item Identifer"@en ;
	skos:broader bdr:BibliographicIdentifier ;
	skos:definition "An identifier associated with an Item"@en ;
	.

bdr:KDPPOldId
	a
		bdo:Identifier ,
		skos:Concept
		;
	rdfs:label "KDPPOld Id"@en ;
	skos:broader bdr:InstanceIdentifier ;
	skos:definition "Khmer Digital Preservation Project Old Id"@en ;
	.

bdr:KaTenSiglaA
	a
		bdo:Identifier ,
		skos:Concept
		;
	rdfs:label "Pedurma catalogue number"@en ;
	rdfs:seeAlso <http://www.worldcat.org/oclc/756377542> ;
	skos:broader bdr:KaTenSiglaIdentifier ;
	skos:definition "From Paul Hackett's catalogue"@en ;
	.

bdr:KaTenSiglaBon
	a
		bdo:Identifier ,
		skos:Concept
		;
	rdfs:label "Bon Katen catalog number"@en ;
	skos:broader bdr:KaTenSiglaIdentifier ;
	skos:definition "Reference number in the Bon Katen"@en ;
	.

bdr:KaTenSiglaC
	a
		bdo:Identifier ,
		skos:Concept
		;
	rdfs:label "Cone catalogue number"@en ;
	rdfs:seeAlso <http://www.worldcat.org/oclc/603601029> ;
	skos:broader bdr:KaTenSiglaIdentifier ;
	skos:definition "from Mibu's catalogue"@en ;
	.

bdr:KaTenSiglaCx
	a
		bdo:Identifier ,
		skos:Concept
		;
	rdfs:label "Golden Mustang Kangyur reference number"@en ;
	skos:broader bdr:KaTenSiglaIdentifier ;
	skos:definition "from rKTs"@en ;
	.

bdr:KaTenSiglaD
	a
		bdo:Identifier ,
		skos:Concept
		;
	rdfs:label "Tohoku catalogue number"@en ;
	rdfs:seeAlso <http://www.worldcat.org/oclc/976594525> ;
	skos:broader bdr:KaTenSiglaIdentifier ;
	skos:definition "Derge Kangyur and Tengyur reference numbers, from the Tohoku Catalogue"@en ;
	.

bdr:KaTenSiglaDo
	a
		bdo:Identifier ,
		skos:Concept
		;
	rdfs:label "Dolpo Kangyur Number"@en ;
	skos:broader bdr:KaTenSiglaIdentifier ;
	skos:definition "Reference number for this work from the Dolpo Kangyur"@en ;
	.

bdr:KaTenSiglaEg
	a
		bdo:Identifier ,
		skos:Concept
		;
	rdfs:label "Egoo Canonical Collection Number"@en ;
	skos:broader bdr:KaTenSiglaIdentifier ;
	skos:definition "Reference number for this work from the Egoo Canonical Collection"@en ;
	.

bdr:KaTenSiglaF
	a
		bdo:Identifier ,
		skos:Concept
		;
	rdfs:label "Phugdrak Kangyur Number"@en ;
	skos:broader bdr:KaTenSiglaIdentifier ;
	skos:definition "Reference number for this work from the Phugdrak Kangyur"@en ;
	.

bdr:KaTenSiglaG
	a
		bdo:Identifier ,
		skos:Concept
		;
	rdfs:label "Ganden Kangyur reference number"@en ;
	skos:broader bdr:KaTenSiglaIdentifier ;
	skos:definition "Ganden (dga’ ldan) or “Golden Manuscript” (gser bris ma) Tengyur reference number"@en ;
	.

bdr:KaTenSiglaH
	a
		bdo:Identifier ,
		skos:Concept
		;
	rdfs:label "Lhasa Kangyur number"@en ;
	skos:broader bdr:KaTenSiglaIdentifier ;
	skos:definition "Lhasa Kanjur reference number"@en ;
	.

bdr:KaTenSiglaHe
	a
		bdo:Identifier ,
		skos:Concept
		;
	rdfs:label "Hemis Kangyur (I) reference number"@en ;
	skos:broader bdr:KaTenSiglaIdentifier ;
	skos:definition "from rKTs"@en ;
	.

bdr:KaTenSiglaIdentifier
	a
		bdo:Identifier ,
		skos:Concept
		;
	rdfs:label "KaTen Sigla Identifer"@en ;
	skos:broader bdr:InstanceIdentifier ;
	skos:definition "An identifier associated with a KaTen Instance"@en ;
	.

bdr:KaTenSiglaJ
	a
		bdo:Identifier ,
		skos:Concept
		;
	rdfs:label "Jang catalogue number"@en ;
	rdfs:seeAlso <http://www.worldcat.org/oclc/769115653> ;
	skos:broader bdr:KaTenSiglaIdentifier ;
	skos:definition "From Imaeda's catalogue"@en ;
	.

bdr:KaTenSiglaN
	a
		bdo:Identifier ,
		skos:Concept
		;
	rdfs:label "Narthang number"@en ;
	rdfs:seeAlso <http://www.worldcat.org/oclc/718065580> ;
	skos:broader bdr:KaTenSiglaIdentifier ;
	skos:definition "Narthang Kangyur and Tengyur reference number, from Eimer's catalogue"@en ;
	.

bdr:KaTenSiglaQ
	a
		bdo:Identifier ,
		skos:Concept
		;
	rdfs:label "Otani catalogue reference"@en ;
	skos:broader bdr:KaTenSiglaIdentifier ;
	skos:definition "Pecing Kangyur Reference number from the Otani catalogue"@en ;
	.

bdr:KaTenSiglaS
	a
		bdo:Identifier ,
		skos:Concept
		;
	rdfs:label "Stog catalogue number"@en ;
	rdfs:seeAlso <http://www.worldcat.org/oclc/461960048> ;
	skos:broader bdr:KaTenSiglaIdentifier ;
	skos:definition "Reference number from Skorupski's catalogue"@en ;
	.

bdr:KaTenSiglaU
	a
		bdo:Identifier ,
		skos:Concept
		;
	rdfs:label "Urga catalogue number"@en ;
	skos:broader bdr:KaTenSiglaIdentifier ;
	skos:definition "Urga Kangyur reference number"@en ;
	.

bdr:KaTenSiglaV
	a
		bdo:Identifier ,
		skos:Concept
		;
	rdfs:label "Ulaanbaatar catalogue number"@en ;
	skos:broader bdr:KaTenSiglaIdentifier ;
	skos:definition "Reference number from the Ulaanbaatar Kangyur"@en ;
	.

bdr:KaTenSiglaZ
	a
		bdo:Identifier ,
		skos:Concept
		;
	rdfs:label "Shey number"@en ;
	rdfs:seeAlso <https://www.istb.univie.ac.at/kanjur/xml4/sub/sigla.php> ;
	skos:broader bdr:KaTenSiglaIdentifier ;
	skos:definition "Shey Palace manuscript reference number"@en ;
	.

bdr:LTWAId
	a
		bdo:Identifier ,
		skos:Concept
		;
	skos:broader bdr:ItemIdentifier ;
	skos:prefLabel "LTWA Accession Number"@en ;
	.

bdr:MARCCountryCode
	a
		bdo:Identifier ,
		skos:Concept
		;
	rdfs:label "MARC Country Code"@en ;
	rdfs:seeAlso
		<http://id.loc.gov/vocabulary/countries.html> ,
		<http://www.loc.gov/marc/countries/>
		;
	skos:broader bdr:PlaceIdentifier ;
	skos:definition "two- or three-character lowercase alphabetic codes that designate countries and regions (such as states in the U.S.)"@en ;
	skos:historyNote "Was bdo:placeMARCCountryCode."@en ;
	.

bdr:NLMId
	a
		bdo:Identifier ,
		skos:Concept
		;
	skos:broader bdr:ItemIdentifier ;
	skos:prefLabel "National Library of Mongolia Accession Number"@en ;
	.

bdr:OclcControlNumber
	a
		bdo:Identifier ,
		skos:Concept
		;
	rdfs:label "OCLC Control Number (OCN)"@en ;
	skos:broader bdr:InstanceIdentifier ;
	.

bdr:PL480
	a
		bdo:Identifier ,
		skos:Concept
		;
	rdfs:label "LOC overseas acq no."@en ;
	skos:broader bdr:InstanceIdentifier ;
	skos:definition "Indicates the overseas acquisition number at Library of Congress."@en ;
	skos:editorialNote "Do not fill for works not created by Gene in the PL480 period. Should be replaced with bf:LcOverseasAcq ."@en ;
	.

bdr:PlaceIdentifier
	a
		bdo:Identifier ,
		skos:Concept
		;
	rdfs:label "Place Identifer"@en ;
	skos:definition "An identifier associated with a Place"@en ;
	skos:topConceptOf bdr:IdentifierScheme ;
	.

bdr:RefCPN
	a
		bdo:Identifier ,
		skos:Concept
		;
	rdfs:label "CPN number"@en ;
	skos:broader bdr:InstanceIdentifier ;
	skos:definition "Chinese Palace of Nationalities Number"@en ;
	.

bdr:RefChokLing
	a
		bdo:Identifier ,
		skos:Concept
		;
	rdfs:label "chokling tersar reference"@en ;
	rdfs:seeAlso "http://rywiki.tsadra.org/index.php/Catalogue_of_the_New_Treasures_of_Chokgyur_Lingpa_Part_1"^^xsd:anyURI ;
	skos:broader bdr:InstanceIdentifier ;
	skos:definition "Catalogue of the New Treasures of Chokgyur Lingpa reference used only in cataloguing parts of bdr:W22642"@en ;
	skos:historyNote "Was bdo:workRefChokLing."@en ;
	.

bdr:RefIsIAO
	a
		bdo:Identifier ,
		skos:Concept
		;
	rdfs:label "IsIAO reference"@en ;
	rdfs:seeAlso bdr:W19841 ;
	skos:broader bdr:InstanceIdentifier ;
	skos:definition "Catalog of the Tucci Tibetan fund in the library of ISMEO"@en ;
	skos:historyNote "Was bdo:workRefIsIAO."@en ;
	.

bdr:RefNCLK
	a
		bdo:Identifier ,
		skos:Concept
		;
	rdfs:label "Drepung number"@en ;
	skos:broader bdr:InstanceIdentifier ;
	skos:definition "See bdr:PR1NCLK"@en ;
	.

bdr:RefrKTsG
	a
		bdo:Identifier ,
		skos:Concept
		;
	rdfs:label "rKTs rnying rgyud reference"@en ;
	rdfs:seeAlso "https://www.istb.univie.ac.at/kanjur/rktsneu/sub/index.php"^^xsd:anyURI ;
	skos:broader bdr:RefrKTsIdentifier ;
	skos:definition "University of Vienna, resources for Kanjur and Tanjur studies (rKTs) reference for a rnying rgyud text"@en ;
	skos:historyNote "Was bdo:workRefrKTsG."@en ;
	.

bdr:RefrKTsIdentifier
	a
		bdo:Identifier ,
		skos:Concept
		;
	rdfs:label "rKTs Identifer"@en ;
	skos:broader bdr:WorkIdentifier ;
	skos:definition "An identifier associated with an rKTs Work"@en ;
	.

bdr:RefrKTsK
	a
		bdo:Identifier ,
		skos:Concept
		;
	rdfs:label "rKTs Kangyur reference"@en ;
	rdfs:seeAlso "https://www.istb.univie.ac.at/kanjur/rktsneu/sub/index.php"^^xsd:anyURI ;
	skos:broader bdr:RefrKTsIdentifier ;
	skos:definition "University of Vienna, resources for Kanjur and Tanjur studies (rKTs) reference number for Kangyur texts"@en ;
	skos:historyNote "Was bdo:workRefrKTsK."@en ;
	.

bdr:RefrKTsT
	a
		bdo:Identifier ,
		skos:Concept
		;
	rdfs:label "rKTs Tengyur reference"@en ;
	rdfs:seeAlso "https://www.istb.univie.ac.at/kanjur/rktsneu/sub/index.php"^^xsd:anyURI ;
	skos:broader bdr:RefrKTsIdentifier ;
	skos:definition "University of Vienna, resources for Kanjur and Tanjur studies (rKTs) reference for a Tengyur text"@en ;
	skos:historyNote "Was bdo:workRefrKTsT."@en ;
	.

bdr:WDSBB
	a
		bdo:Identifier ,
		skos:Concept
		;
	rdfs:label "Waddell"@en ;
	skos:broader bdr:InstanceIdentifier ;
	skos:definition "Indicates the Waddell identifier in the collection at the Stabi in Berlin"@en ;
	.

bdr:WorkIdentifier
	a
		bdo:Identifier ,
		skos:Concept
		;
	rdfs:label "Work Identifer"@en ;
	skos:broader bdr:BibliographicIdentifier ;
	skos:definition "An identifier associated with a Work"@en ;
	.

